refactor: rename timeOrder for CrAnAlgebra

HepLean/PerturbationTheory/Algebras/CrAnAlgebra/TimeOrder.lean
@@ -27,19 +27,19 @@ open HepLean.List
 -/
 
 /-- Time ordering for the `CrAnAlgebra`. -/
-def timeOrder : CrAnAlgebra 𝓕 →ₗ[ℂ] CrAnAlgebra 𝓕 :=
+def timeOrderF : CrAnAlgebra 𝓕 →ₗ[ℂ] CrAnAlgebra 𝓕 :=
   Basis.constr ofCrAnListBasis ℂ fun φs =>
   crAnTimeOrderSign φs • ofCrAnList (crAnTimeOrderList φs)
 
-@[inherit_doc timeOrder]
-scoped[FieldSpecification.CrAnAlgebra] notation "𝓣ᶠ(" a ")" => timeOrder a
+@[inherit_doc timeOrderF]
+scoped[FieldSpecification.CrAnAlgebra] notation "𝓣ᶠ(" a ")" => timeOrderF a
 
-lemma timeOrder_ofCrAnList (φs : List 𝓕.CrAnStates) :
+lemma timeOrderF_ofCrAnList (φs : List 𝓕.CrAnStates) :
     𝓣ᶠ(ofCrAnList φs) = crAnTimeOrderSign φs • ofCrAnList (crAnTimeOrderList φs) := by
   rw [← ofListBasis_eq_ofList]
-  simp only [timeOrder, Basis.constr_basis]
+  simp only [timeOrderF, Basis.constr_basis]
 
-lemma timeOrder_timeOrder_mid (a b c : 𝓕.CrAnAlgebra) : 𝓣ᶠ(a * b * c) = 𝓣ᶠ(a * 𝓣ᶠ(b) * c) := by
+lemma timeOrderF_timeOrderF_mid (a b c : 𝓕.CrAnAlgebra) : 𝓣ᶠ(a * b * c) = 𝓣ᶠ(a * 𝓣ᶠ(b) * c) := by
   let pc (c : 𝓕.CrAnAlgebra) (hc : c ∈ Submodule.span ℂ (Set.range ofCrAnListBasis)) :
     Prop := 𝓣ᶠ(a * b * c) = 𝓣ᶠ(a * 𝓣ᶠ(b) * c)
   change pc c (Basis.mem_span _ c)
@@ -61,10 +61,10 @@ lemma timeOrder_timeOrder_mid (a b c : 𝓕.CrAnAlgebra) : 𝓣ᶠ(a * b * c) = 
       · intro x hx
         obtain ⟨φs'', rfl⟩ := hx
         simp only [ofListBasis_eq_ofList, pa]
-        rw [timeOrder_ofCrAnList]
+        rw [timeOrderF_ofCrAnList]
         simp only [← ofCrAnList_append, Algebra.mul_smul_comm,
           Algebra.smul_mul_assoc, map_smul]
-        rw [timeOrder_ofCrAnList, timeOrder_ofCrAnList, smul_smul]
+        rw [timeOrderF_ofCrAnList, timeOrderF_ofCrAnList, smul_smul]
         congr 1
         · simp only [crAnTimeOrderSign, crAnTimeOrderList]
           rw [Wick.koszulSign_of_append_eq_insertionSort, mul_comm]
@@ -87,68 +87,68 @@ lemma timeOrder_timeOrder_mid (a b c : 𝓕.CrAnAlgebra) : 𝓣ᶠ(a * b * c) = 
   · intro x hx h hp
     simp_all [pc]
 
-lemma timeOrder_timeOrder_right (a b : 𝓕.CrAnAlgebra) : 𝓣ᶠ(a * b) = 𝓣ᶠ(a * 𝓣ᶠ(b)) := by
+lemma timeOrderF_timeOrderF_right (a b : 𝓕.CrAnAlgebra) : 𝓣ᶠ(a * b) = 𝓣ᶠ(a * 𝓣ᶠ(b)) := by
   trans 𝓣ᶠ(a * b * 1)
   · simp
-  · rw [timeOrder_timeOrder_mid]
+  · rw [timeOrderF_timeOrderF_mid]
     simp
 
-lemma timeOrder_timeOrder_left (a b : 𝓕.CrAnAlgebra) : 𝓣ᶠ(a * b) = 𝓣ᶠ(𝓣ᶠ(a) * b) := by
+lemma timeOrderF_timeOrderF_left (a b : 𝓕.CrAnAlgebra) : 𝓣ᶠ(a * b) = 𝓣ᶠ(𝓣ᶠ(a) * b) := by
   trans 𝓣ᶠ(1 * a * b)
   · simp
-  · rw [timeOrder_timeOrder_mid]
+  · rw [timeOrderF_timeOrderF_mid]
     simp
 
-lemma timeOrder_ofStateList (φs : List 𝓕.States) :
+lemma timeOrderF_ofStateList (φs : List 𝓕.States) :
     𝓣ᶠ(ofStateList φs) = timeOrderSign φs • ofStateList (timeOrderList φs) := by
   conv_lhs =>
     rw [ofStateList_sum, map_sum]
     enter [2, x]
-    rw [timeOrder_ofCrAnList]
+    rw [timeOrderF_ofCrAnList]
   simp only [crAnTimeOrderSign_crAnSection]
   rw [← Finset.smul_sum]
   congr
   rw [ofStateList_sum, sum_crAnSections_timeOrder]
   rfl
 
-lemma timeOrder_ofStateList_nil : timeOrder (𝓕 := 𝓕) (ofStateList []) = 1 := by
-  rw [timeOrder_ofStateList]
+lemma timeOrderF_ofStateList_nil : timeOrderF (𝓕 := 𝓕) (ofStateList []) = 1 := by
+  rw [timeOrderF_ofStateList]
   simp [timeOrderSign, Wick.koszulSign, timeOrderList]
 
 @[simp]
-lemma timeOrder_ofStateList_singleton (φ : 𝓕.States) : 𝓣ᶠ(ofStateList [φ]) = ofStateList [φ] := by
-  simp [timeOrder_ofStateList, timeOrderSign, timeOrderList]
+lemma timeOrderF_ofStateList_singleton (φ : 𝓕.States) : 𝓣ᶠ(ofStateList [φ]) = ofStateList [φ] := by
+  simp [timeOrderF_ofStateList, timeOrderSign, timeOrderList]
 
-lemma timeOrder_ofState_ofState_ordered {φ ψ : 𝓕.States} (h : timeOrderRel φ ψ) :
+lemma timeOrderF_ofState_ofState_ordered {φ ψ : 𝓕.States} (h : timeOrderRel φ ψ) :
     𝓣ᶠ(ofState φ * ofState ψ) = ofState φ * ofState ψ := by
-  rw [← ofStateList_singleton, ← ofStateList_singleton, ← ofStateList_append, timeOrder_ofStateList]
+  rw [← ofStateList_singleton, ← ofStateList_singleton, ← ofStateList_append, timeOrderF_ofStateList]
   simp only [List.singleton_append]
   rw [timeOrderSign_pair_ordered h, timeOrderList_pair_ordered h]
   simp
 
-lemma timeOrder_ofState_ofState_not_ordered {φ ψ : 𝓕.States} (h : ¬ timeOrderRel φ ψ) :
+lemma timeOrderF_ofState_ofState_not_ordered {φ ψ : 𝓕.States} (h : ¬ timeOrderRel φ ψ) :
     𝓣ᶠ(ofState φ * ofState ψ) = 𝓢(𝓕 |>ₛ φ, 𝓕 |>ₛ ψ) • ofState ψ * ofState φ := by
   rw [← ofStateList_singleton, ← ofStateList_singleton,
-    ← ofStateList_append, timeOrder_ofStateList]
+    ← ofStateList_append, timeOrderF_ofStateList]
   simp only [List.singleton_append, instCommGroup.eq_1, Algebra.smul_mul_assoc]
   rw [timeOrderSign_pair_not_ordered h, timeOrderList_pair_not_ordered h]
   simp [← ofStateList_append]
 
-lemma timeOrder_ofState_ofState_not_ordered_eq_timeOrder {φ ψ : 𝓕.States} (h : ¬ timeOrderRel φ ψ) :
+lemma timeOrderF_ofState_ofState_not_ordered_eq_timeOrderF {φ ψ : 𝓕.States} (h : ¬ timeOrderRel φ ψ) :
     𝓣ᶠ(ofState φ * ofState ψ) = 𝓢(𝓕 |>ₛ φ, 𝓕 |>ₛ ψ) • 𝓣ᶠ(ofState ψ * ofState φ) := by
-  rw [timeOrder_ofState_ofState_not_ordered h]
-  rw [timeOrder_ofState_ofState_ordered]
+  rw [timeOrderF_ofState_ofState_not_ordered h]
+  rw [timeOrderF_ofState_ofState_ordered]
   simp only [instCommGroup.eq_1, Algebra.smul_mul_assoc]
   have hx := IsTotal.total (r := timeOrderRel) ψ φ
   simp_all
 
-lemma timeOrder_superCommuteF_ofCrAnState_ofCrAnState_not_crAnTimeOrderRel
+lemma timeOrderF_superCommuteF_ofCrAnState_ofCrAnState_not_crAnTimeOrderRel
     {φ ψ : 𝓕.CrAnStates} (h : ¬ crAnTimeOrderRel φ ψ) :
     𝓣ᶠ([ofCrAnState φ, ofCrAnState ψ]ₛca) = 0 := by
   rw [superCommuteF_ofCrAnState_ofCrAnState]
   simp only [instCommGroup.eq_1, Algebra.smul_mul_assoc, map_sub, map_smul]
   rw [← ofCrAnList_singleton, ← ofCrAnList_singleton,
-    ← ofCrAnList_append, ← ofCrAnList_append, timeOrder_ofCrAnList, timeOrder_ofCrAnList]
+    ← ofCrAnList_append, ← ofCrAnList_append, timeOrderF_ofCrAnList, timeOrderF_ofCrAnList]
   simp only [List.singleton_append]
   rw [crAnTimeOrderSign_pair_not_ordered h, crAnTimeOrderList_pair_not_ordered h]
   rw [sub_eq_zero, smul_smul]
@@ -160,51 +160,51 @@ lemma timeOrder_superCommuteF_ofCrAnState_ofCrAnState_not_crAnTimeOrderRel
   · rw [crAnTimeOrderList_pair_ordered]
     simp_all
 
-lemma timeOrder_superCommuteF_ofCrAnState_ofCrAnState_not_crAnTimeOrderRel_right
+lemma timeOrderF_superCommuteF_ofCrAnState_ofCrAnState_not_crAnTimeOrderRel_right
     {φ ψ : 𝓕.CrAnStates} (h : ¬ crAnTimeOrderRel φ ψ) (a : 𝓕.CrAnAlgebra) :
     𝓣ᶠ(a * [ofCrAnState φ, ofCrAnState ψ]ₛca) = 0 := by
-  rw [timeOrder_timeOrder_right,
-    timeOrder_superCommuteF_ofCrAnState_ofCrAnState_not_crAnTimeOrderRel h]
+  rw [timeOrderF_timeOrderF_right,
+    timeOrderF_superCommuteF_ofCrAnState_ofCrAnState_not_crAnTimeOrderRel h]
   simp
 
-lemma timeOrder_superCommuteF_ofCrAnState_ofCrAnState_not_crAnTimeOrderRel_left
+lemma timeOrderF_superCommuteF_ofCrAnState_ofCrAnState_not_crAnTimeOrderRel_left
     {φ ψ : 𝓕.CrAnStates} (h : ¬ crAnTimeOrderRel φ ψ) (a : 𝓕.CrAnAlgebra) :
     𝓣ᶠ([ofCrAnState φ, ofCrAnState ψ]ₛca * a) = 0 := by
-  rw [timeOrder_timeOrder_left,
-    timeOrder_superCommuteF_ofCrAnState_ofCrAnState_not_crAnTimeOrderRel h]
+  rw [timeOrderF_timeOrderF_left,
+    timeOrderF_superCommuteF_ofCrAnState_ofCrAnState_not_crAnTimeOrderRel h]
   simp
 
-lemma timeOrder_superCommuteF_ofCrAnState_ofCrAnState_not_crAnTimeOrderRel_mid
+lemma timeOrderF_superCommuteF_ofCrAnState_ofCrAnState_not_crAnTimeOrderRel_mid
     {φ ψ : 𝓕.CrAnStates} (h : ¬ crAnTimeOrderRel φ ψ) (a b : 𝓕.CrAnAlgebra) :
     𝓣ᶠ(a * [ofCrAnState φ, ofCrAnState ψ]ₛca * b) = 0 := by
-  rw [timeOrder_timeOrder_mid,
-    timeOrder_superCommuteF_ofCrAnState_ofCrAnState_not_crAnTimeOrderRel h]
+  rw [timeOrderF_timeOrderF_mid,
+    timeOrderF_superCommuteF_ofCrAnState_ofCrAnState_not_crAnTimeOrderRel h]
   simp
 
-lemma timeOrder_superCommuteF_superCommuteF_ofCrAnState_not_crAnTimeOrderRel
+lemma timeOrderF_superCommuteF_superCommuteF_ofCrAnState_not_crAnTimeOrderRel
     {φ1 φ2 : 𝓕.CrAnStates} (h : ¬ crAnTimeOrderRel φ1 φ2) (a : 𝓕.CrAnAlgebra) :
     𝓣ᶠ([a, [ofCrAnState φ1, ofCrAnState φ2]ₛca]ₛca) = 0 := by
   rw [← bosonicProj_add_fermionicProj a]
   simp only [map_add, LinearMap.add_apply]
   rw [bosonic_superCommuteF (Submodule.coe_mem (bosonicProj a))]
   simp only [map_sub]
-  rw [timeOrder_superCommuteF_ofCrAnState_ofCrAnState_not_crAnTimeOrderRel_left h]
-  rw [timeOrder_superCommuteF_ofCrAnState_ofCrAnState_not_crAnTimeOrderRel_right h]
+  rw [timeOrderF_superCommuteF_ofCrAnState_ofCrAnState_not_crAnTimeOrderRel_left h]
+  rw [timeOrderF_superCommuteF_ofCrAnState_ofCrAnState_not_crAnTimeOrderRel_right h]
   simp only [sub_self, zero_add]
   rw [← ofCrAnList_singleton, ← ofCrAnList_singleton]
   rcases superCommuteF_ofCrAnList_ofCrAnList_bosonic_or_fermionic [φ1] [φ2] with h' | h'
   · rw [superCommuteF_bonsonic h']
     simp only [ofCrAnList_singleton, map_sub]
-    rw [timeOrder_superCommuteF_ofCrAnState_ofCrAnState_not_crAnTimeOrderRel_left h]
-    rw [timeOrder_superCommuteF_ofCrAnState_ofCrAnState_not_crAnTimeOrderRel_right h]
+    rw [timeOrderF_superCommuteF_ofCrAnState_ofCrAnState_not_crAnTimeOrderRel_left h]
+    rw [timeOrderF_superCommuteF_ofCrAnState_ofCrAnState_not_crAnTimeOrderRel_right h]
     simp
   · rw [superCommuteF_fermionic_fermionic (Submodule.coe_mem (fermionicProj a)) h']
     simp only [ofCrAnList_singleton, map_add]
-    rw [timeOrder_superCommuteF_ofCrAnState_ofCrAnState_not_crAnTimeOrderRel_left h]
-    rw [timeOrder_superCommuteF_ofCrAnState_ofCrAnState_not_crAnTimeOrderRel_right h]
+    rw [timeOrderF_superCommuteF_ofCrAnState_ofCrAnState_not_crAnTimeOrderRel_left h]
+    rw [timeOrderF_superCommuteF_ofCrAnState_ofCrAnState_not_crAnTimeOrderRel_right h]
     simp
 
-lemma timeOrder_superCommuteF_ofCrAnState_superCommuteF_not_crAnTimeOrderRel
+lemma timeOrderF_superCommuteF_ofCrAnState_superCommuteF_not_crAnTimeOrderRel
     {φ1 φ2 φ3 : 𝓕.CrAnStates} (h12 : ¬ crAnTimeOrderRel φ1 φ2)
     (h13 : ¬ crAnTimeOrderRel φ1 φ3) :
     𝓣ᶠ([ofCrAnState φ1, [ofCrAnState φ2, ofCrAnState φ3]ₛca]ₛca) = 0 := by
@@ -213,14 +213,14 @@ lemma timeOrder_superCommuteF_ofCrAnState_superCommuteF_not_crAnTimeOrderRel
   simp only [instCommGroup.eq_1, ofList_singleton, ofCrAnList_singleton, neg_smul, map_smul,
     map_sub, map_neg, smul_eq_zero]
   right
-  rw [timeOrder_superCommuteF_superCommuteF_ofCrAnState_not_crAnTimeOrderRel h12]
+  rw [timeOrderF_superCommuteF_superCommuteF_ofCrAnState_not_crAnTimeOrderRel h12]
   rw [superCommuteF_ofCrAnState_ofCrAnState_symm φ3]
   simp only [smul_zero, neg_zero, instCommGroup.eq_1, neg_smul, map_neg, map_smul, smul_neg,
     sub_neg_eq_add, zero_add, smul_eq_zero]
-  rw [timeOrder_superCommuteF_superCommuteF_ofCrAnState_not_crAnTimeOrderRel h13]
+  rw [timeOrderF_superCommuteF_superCommuteF_ofCrAnState_not_crAnTimeOrderRel h13]
   simp
 
-lemma timeOrder_superCommuteF_ofCrAnState_superCommuteF_not_crAnTimeOrderRel'
+lemma timeOrderF_superCommuteF_ofCrAnState_superCommuteF_not_crAnTimeOrderRel'
     {φ1 φ2 φ3 : 𝓕.CrAnStates} (h12 : ¬ crAnTimeOrderRel φ2 φ1)
     (h13 : ¬ crAnTimeOrderRel φ3 φ1) :
     𝓣ᶠ([ofCrAnState φ1, [ofCrAnState φ2, ofCrAnState φ3]ₛca]ₛca) = 0 := by
@@ -231,12 +231,12 @@ lemma timeOrder_superCommuteF_ofCrAnState_superCommuteF_not_crAnTimeOrderRel'
   right
   rw [superCommuteF_ofCrAnState_ofCrAnState_symm φ1]
   simp only [instCommGroup.eq_1, neg_smul, map_neg, map_smul, smul_neg, neg_neg]
-  rw [timeOrder_superCommuteF_superCommuteF_ofCrAnState_not_crAnTimeOrderRel h12]
+  rw [timeOrderF_superCommuteF_superCommuteF_ofCrAnState_not_crAnTimeOrderRel h12]
   simp only [smul_zero, zero_sub, neg_eq_zero, smul_eq_zero]
-  rw [timeOrder_superCommuteF_superCommuteF_ofCrAnState_not_crAnTimeOrderRel h13]
+  rw [timeOrderF_superCommuteF_superCommuteF_ofCrAnState_not_crAnTimeOrderRel h13]
   simp
 
-lemma timeOrder_superCommuteF_ofCrAnState_superCommuteF_all_not_crAnTimeOrderRel
+lemma timeOrderF_superCommuteF_ofCrAnState_superCommuteF_all_not_crAnTimeOrderRel
     (φ1 φ2 φ3 : 𝓕.CrAnStates) (h : ¬
       (crAnTimeOrderRel φ1 φ2 ∧ crAnTimeOrderRel φ1 φ3 ∧
       crAnTimeOrderRel φ2 φ1 ∧ crAnTimeOrderRel φ2 φ3 ∧
@@ -245,13 +245,13 @@ lemma timeOrder_superCommuteF_ofCrAnState_superCommuteF_all_not_crAnTimeOrderRel
   simp only [not_and] at h
   by_cases h23 : ¬ crAnTimeOrderRel φ2 φ3
   · simp_all only [IsEmpty.forall_iff, implies_true]
-    rw [timeOrder_superCommuteF_superCommuteF_ofCrAnState_not_crAnTimeOrderRel h23]
+    rw [timeOrderF_superCommuteF_superCommuteF_ofCrAnState_not_crAnTimeOrderRel h23]
   simp_all only [Decidable.not_not, forall_const]
   by_cases h32 : ¬ crAnTimeOrderRel φ3 φ2
   · simp_all only [not_false_eq_true, implies_true]
     rw [superCommuteF_ofCrAnState_ofCrAnState_symm]
     simp only [instCommGroup.eq_1, neg_smul, map_neg, map_smul, neg_eq_zero, smul_eq_zero]
-    rw [timeOrder_superCommuteF_superCommuteF_ofCrAnState_not_crAnTimeOrderRel h32]
+    rw [timeOrderF_superCommuteF_superCommuteF_ofCrAnState_not_crAnTimeOrderRel h32]
     simp
   simp_all only [imp_false, Decidable.not_not]
   by_cases h12 : ¬ crAnTimeOrderRel φ1 φ2
@@ -259,7 +259,7 @@ lemma timeOrder_superCommuteF_ofCrAnState_superCommuteF_all_not_crAnTimeOrderRel
       intro h13
       apply h12
       exact IsTrans.trans φ1 φ3 φ2 h13 h32
-    rw [timeOrder_superCommuteF_ofCrAnState_superCommuteF_not_crAnTimeOrderRel h12 h13]
+    rw [timeOrderF_superCommuteF_ofCrAnState_superCommuteF_not_crAnTimeOrderRel h12 h13]
   simp_all only [Decidable.not_not, forall_const]
   have h13 : crAnTimeOrderRel φ1 φ3 := IsTrans.trans φ1 φ2 φ3 h12 h23
   simp_all only [forall_const]
@@ -269,18 +269,18 @@ lemma timeOrder_superCommuteF_ofCrAnState_superCommuteF_all_not_crAnTimeOrderRel
       intro h31
       apply h21
       exact IsTrans.trans φ2 φ3 φ1 h23 h31
-    rw [timeOrder_superCommuteF_ofCrAnState_superCommuteF_not_crAnTimeOrderRel' h21 h31]
+    rw [timeOrderF_superCommuteF_ofCrAnState_superCommuteF_not_crAnTimeOrderRel' h21 h31]
   simp_all only [Decidable.not_not, forall_const]
   refine False.elim (h ?_)
   exact IsTrans.trans φ3 φ2 φ1 h32 h21
 
-lemma timeOrder_superCommuteF_ofCrAnState_ofCrAnState_eq_time
+lemma timeOrderF_superCommuteF_ofCrAnState_ofCrAnState_eq_time
     {φ ψ : 𝓕.CrAnStates} (h1 : crAnTimeOrderRel φ ψ) (h2 : crAnTimeOrderRel ψ φ) :
     𝓣ᶠ([ofCrAnState φ, ofCrAnState ψ]ₛca) = [ofCrAnState φ, ofCrAnState ψ]ₛca := by
   rw [superCommuteF_ofCrAnState_ofCrAnState]
   simp only [instCommGroup.eq_1, Algebra.smul_mul_assoc, map_sub, map_smul]
   rw [← ofCrAnList_singleton, ← ofCrAnList_singleton,
-    ← ofCrAnList_append, ← ofCrAnList_append, timeOrder_ofCrAnList, timeOrder_ofCrAnList]
+    ← ofCrAnList_append, ← ofCrAnList_append, timeOrderF_ofCrAnList, timeOrderF_ofCrAnList]
   simp only [List.singleton_append]
   rw [crAnTimeOrderSign_pair_ordered h1, crAnTimeOrderList_pair_ordered h1,
     crAnTimeOrderSign_pair_ordered h2, crAnTimeOrderList_pair_ordered h2]
@@ -295,12 +295,12 @@ lemma timeOrder_superCommuteF_ofCrAnState_ofCrAnState_eq_time
 /-- In the state algebra time, ordering obeys `T(φ₀φ₁…φₙ) = s * φᵢ * T(φ₀φ₁…φᵢ₋₁φᵢ₊₁…φₙ)`
   where `φᵢ` is the state
   which has maximum time and `s` is the exchange sign of `φᵢ` and `φ₀φ₁…φᵢ₋₁`. -/
-lemma timeOrder_eq_maxTimeField_mul (φ : 𝓕.States) (φs : List 𝓕.States) :
+lemma timeOrderF_eq_maxTimeField_mul (φ : 𝓕.States) (φs : List 𝓕.States) :
     𝓣ᶠ(ofStateList (φ :: φs)) =
     𝓢(𝓕 |>ₛ maxTimeField φ φs, 𝓕 |>ₛ (φ :: φs).take (maxTimeFieldPos φ φs)) •
     ofState (maxTimeField φ φs) * 𝓣ᶠ(ofStateList (eraseMaxTimeField φ φs)) := by
-  rw [timeOrder_ofStateList, timeOrderList_eq_maxTimeField_timeOrderList]
-  rw [ofStateList_cons, timeOrder_ofStateList]
+  rw [timeOrderF_ofStateList, timeOrderList_eq_maxTimeField_timeOrderList]
+  rw [ofStateList_cons, timeOrderF_ofStateList]
   simp only [instCommGroup.eq_1, Algebra.mul_smul_comm, Algebra.smul_mul_assoc, smul_smul]
   congr
   rw [timerOrderSign_of_eraseMaxTimeField, mul_assoc]
@@ -310,12 +310,12 @@ lemma timeOrder_eq_maxTimeField_mul (φ : 𝓕.States) (φs : List 𝓕.States) 
   where `φᵢ` is the state
   which has maximum time and `s` is the exchange sign of `φᵢ` and `φ₀φ₁…φᵢ₋₁`.
   Here `s` is written using finite sets. -/
-lemma timeOrder_eq_maxTimeField_mul_finset (φ : 𝓕.States) (φs : List 𝓕.States) :
+lemma timeOrderF_eq_maxTimeField_mul_finset (φ : 𝓕.States) (φs : List 𝓕.States) :
     𝓣ᶠ(ofStateList (φ :: φs)) = 𝓢(𝓕 |>ₛ maxTimeField φ φs, 𝓕 |>ₛ ⟨(eraseMaxTimeField φ φs).get,
       (Finset.filter (fun x =>
         (maxTimeFieldPosFin φ φs).succAbove x < maxTimeFieldPosFin φ φs) Finset.univ)⟩) •
       ofState (maxTimeField φ φs) * 𝓣ᶠ(ofStateList (eraseMaxTimeField φ φs)) := by
-  rw [timeOrder_eq_maxTimeField_mul]
+  rw [timeOrderF_eq_maxTimeField_mul]
   congr 3
   apply FieldStatistic.ofList_perm
   nth_rewrite 1 [← List.finRange_map_get (φ :: φs)]
