HepLean/PerturbationTheory/Algebras/FieldOpAlgebra/TimeOrder.lean
@@ -19,7 +19,7 @@ open FieldStatistic
 namespace FieldOpAlgebra
 variable {𝓕 : FieldSpecification}
 
-lemma ι_timeOrder_superCommuteF_superCommuteF_eq_time_ofCrAnList {φ1 φ2 φ3 : 𝓕.CrAnStates}
+lemma ι_timeOrderF_superCommuteF_superCommuteF_eq_time_ofCrAnList {φ1 φ2 φ3 : 𝓕.CrAnStates}
     (φs1 φs2 : List 𝓕.CrAnStates) (h :
       crAnTimeOrderRel φ1 φ2 ∧ crAnTimeOrderRel φ1 φ3 ∧
       crAnTimeOrderRel φ2 φ1 ∧ crAnTimeOrderRel φ2 φ3 ∧
@@ -38,7 +38,7 @@ lemma ι_timeOrder_superCommuteF_superCommuteF_eq_time_ofCrAnList {φ1 φ2 φ3 :
       • (ι (ofCrAnList l1) * ι (ofCrAnList [φ1, φ2, φ3]) * ι (ofCrAnList l2)) := by
     have h1 := insertionSort_of_eq_list 𝓕.crAnTimeOrderRel φ1 φs1 [φ1, φ2, φ3] φs2
       (by simp_all)
-    rw [timeOrder_ofCrAnList, show φs1 ++ φ1 :: φ2 :: φ3 :: φs2 = φs1 ++ [φ1, φ2, φ3] ++ φs2
+    rw [timeOrderF_ofCrAnList, show φs1 ++ φ1 :: φ2 :: φ3 :: φs2 = φs1 ++ [φ1, φ2, φ3] ++ φs2
       by simp, crAnTimeOrderList, h1]
     simp only [List.append_assoc, List.singleton_append, decide_not,
       Bool.decide_and, ofCrAnList_append, map_smul, map_mul, l1, l2, mul_assoc]
@@ -47,7 +47,7 @@ lemma ι_timeOrder_superCommuteF_superCommuteF_eq_time_ofCrAnList {φ1 φ2 φ3 :
       • (ι (ofCrAnList l1) * ι (ofCrAnList [φ1, φ3, φ2]) * ι (ofCrAnList l2)) := by
     have h1 := insertionSort_of_eq_list 𝓕.crAnTimeOrderRel φ1 φs1 [φ1, φ3, φ2] φs2
         (by simp_all)
-    rw [timeOrder_ofCrAnList, show φs1 ++ φ1 :: φ3 :: φ2 :: φs2 = φs1 ++ [φ1, φ3, φ2] ++ φs2
+    rw [timeOrderF_ofCrAnList, show φs1 ++ φ1 :: φ3 :: φ2 :: φs2 = φs1 ++ [φ1, φ3, φ2] ++ φs2
       by simp, crAnTimeOrderList, h1]
     simp only [List.singleton_append, decide_not,
       Bool.decide_and, ofCrAnList_append, map_smul, map_mul, l1, l2, mul_assoc]
@@ -72,7 +72,7 @@ lemma ι_timeOrder_superCommuteF_superCommuteF_eq_time_ofCrAnList {φ1 φ2 φ3 :
       • (ι (ofCrAnList l1) * ι (ofCrAnList [φ2, φ3, φ1]) * ι (ofCrAnList l2)) := by
     have h1 := insertionSort_of_eq_list 𝓕.crAnTimeOrderRel φ1 φs1 [φ2, φ3, φ1] φs2
         (by simp_all)
-    rw [timeOrder_ofCrAnList, show φs1 ++ φ2 :: φ3 :: φ1 :: φs2 = φs1 ++ [φ2, φ3, φ1] ++ φs2
+    rw [timeOrderF_ofCrAnList, show φs1 ++ φ2 :: φ3 :: φ1 :: φs2 = φs1 ++ [φ2, φ3, φ1] ++ φs2
       by simp, crAnTimeOrderList, h1]
     simp only [List.singleton_append, decide_not,
       Bool.decide_and, ofCrAnList_append, map_smul, map_mul, l1, l2, mul_assoc]
@@ -90,7 +90,7 @@ lemma ι_timeOrder_superCommuteF_superCommuteF_eq_time_ofCrAnList {φ1 φ2 φ3 :
       • (ι (ofCrAnList l1) * ι (ofCrAnList [φ3, φ2, φ1]) * ι (ofCrAnList l2)) := by
     have h1 := insertionSort_of_eq_list 𝓕.crAnTimeOrderRel φ1 φs1 [φ3, φ2, φ1] φs2
         (by simp_all)
-    rw [timeOrder_ofCrAnList, show φs1 ++ φ3 :: φ2 :: φ1 :: φs2 = φs1 ++ [φ3, φ2, φ1] ++ φs2
+    rw [timeOrderF_ofCrAnList, show φs1 ++ φ3 :: φ2 :: φ1 :: φs2 = φs1 ++ [φ3, φ2, φ1] ++ φs2
       by simp, crAnTimeOrderList, h1]
     simp only [List.singleton_append, decide_not,
       Bool.decide_and, ofCrAnList_append, map_smul, map_mul, l1, l2, mul_assoc]
@@ -139,7 +139,7 @@ lemma ι_timeOrder_superCommuteF_superCommuteF_eq_time_ofCrAnList {φ1 φ2 φ3 :
     map_smul, smul_sub]
   simp_all
 
-lemma ι_timeOrder_superCommuteF_superCommuteF_ofCrAnList {φ1 φ2 φ3 : 𝓕.CrAnStates}
+lemma ι_timeOrderF_superCommuteF_superCommuteF_ofCrAnList {φ1 φ2 φ3 : 𝓕.CrAnStates}
     (φs1 φs2 : List 𝓕.CrAnStates) :
     ι 𝓣ᶠ(ofCrAnList φs1 * [ofCrAnState φ1, [ofCrAnState φ2, ofCrAnState φ3]ₛca]ₛca * ofCrAnList φs2)
     = 0 := by
@@ -147,13 +147,13 @@ lemma ι_timeOrder_superCommuteF_superCommuteF_ofCrAnList {φ1 φ2 φ3 : 𝓕.Cr
       crAnTimeOrderRel φ1 φ2 ∧ crAnTimeOrderRel φ1 φ3 ∧
       crAnTimeOrderRel φ2 φ1 ∧ crAnTimeOrderRel φ2 φ3 ∧
       crAnTimeOrderRel φ3 φ1 ∧ crAnTimeOrderRel φ3 φ2
-  · exact ι_timeOrder_superCommuteF_superCommuteF_eq_time_ofCrAnList φs1 φs2 h
-  · rw [timeOrder_timeOrder_mid]
-    rw [timeOrder_superCommuteF_ofCrAnState_superCommuteF_all_not_crAnTimeOrderRel _ _ _ h]
+  · exact ι_timeOrderF_superCommuteF_superCommuteF_eq_time_ofCrAnList φs1 φs2 h
+  · rw [timeOrderF_timeOrderF_mid]
+    rw [timeOrderF_superCommuteF_ofCrAnState_superCommuteF_all_not_crAnTimeOrderRel _ _ _ h]
     simp
 
 @[simp]
-lemma ι_timeOrder_superCommuteF_superCommuteF {φ1 φ2 φ3 : 𝓕.CrAnStates} (a b : 𝓕.CrAnAlgebra) :
+lemma ι_timeOrderF_superCommuteF_superCommuteF {φ1 φ2 φ3 : 𝓕.CrAnStates} (a b : 𝓕.CrAnAlgebra) :
     ι 𝓣ᶠ(a * [ofCrAnState φ1, [ofCrAnState φ2, ofCrAnState φ3]ₛca]ₛca * b) = 0 := by
   let pb (b : 𝓕.CrAnAlgebra) (hc : b ∈ Submodule.span ℂ (Set.range ofCrAnListBasis)) :
     Prop := ι 𝓣ᶠ(a * [ofCrAnState φ1, [ofCrAnState φ2, ofCrAnState φ3]ₛca]ₛca * b) = 0
@@ -169,7 +169,7 @@ lemma ι_timeOrder_superCommuteF_superCommuteF {φ1 φ2 φ3 : 𝓕.CrAnStates} (
     · intro x hx
       obtain ⟨φs', rfl⟩ := hx
       simp only [ofListBasis_eq_ofList, pa]
-      exact ι_timeOrder_superCommuteF_superCommuteF_ofCrAnList φs' φs
+      exact ι_timeOrderF_superCommuteF_superCommuteF_ofCrAnList φs' φs
     · simp [pa]
     · intro x y hx hy hpx hpy
       simp_all [pa,mul_add, add_mul]
@@ -181,7 +181,7 @@ lemma ι_timeOrder_superCommuteF_superCommuteF {φ1 φ2 φ3 : 𝓕.CrAnStates} (
   · intro x hx hpx
     simp_all [pb, hpx]
 
-lemma ι_timeOrder_superCommuteF_eq_time {φ ψ : 𝓕.CrAnStates}
+lemma ι_timeOrderF_superCommuteF_eq_time {φ ψ : 𝓕.CrAnStates}
     (hφψ : crAnTimeOrderRel φ ψ) (hψφ : crAnTimeOrderRel ψ φ) (a b : 𝓕.CrAnAlgebra) :
     ι 𝓣ᶠ(a * [ofCrAnState φ, ofCrAnState ψ]ₛca * b) =
     ι ([ofCrAnState φ, ofCrAnState ψ]ₛca * 𝓣ᶠ(a * b)) := by
@@ -204,7 +204,7 @@ lemma ι_timeOrder_superCommuteF_eq_time {φ ψ : 𝓕.CrAnStates}
       conv_lhs =>
         rw [← ofCrAnList_singleton, ← ofCrAnList_singleton, superCommuteF_ofCrAnList_ofCrAnList]
         simp [mul_sub, sub_mul, ← ofCrAnList_append]
-        rw [timeOrder_ofCrAnList, timeOrder_ofCrAnList]
+        rw [timeOrderF_ofCrAnList, timeOrderF_ofCrAnList]
       have h1 : crAnTimeOrderSign (φs' ++ φ :: ψ :: φs) =
           crAnTimeOrderSign (φs' ++ ψ :: φ :: φs) := by
         trans crAnTimeOrderSign (φs' ++ [φ, ψ] ++ φs)
@@ -260,7 +260,7 @@ lemma ι_timeOrder_superCommuteF_eq_time {φ ψ : 𝓕.CrAnStates}
       · rw [ι_superCommuteF_of_diff_statistic hq]
         simp
       · rw [crAnTimeOrderSign, Wick.koszulSign_eq_rel_eq_stat _ _, ← crAnTimeOrderSign]
-        rw [timeOrder_ofCrAnList]
+        rw [timeOrderF_ofCrAnList]
         simp only [map_smul, Algebra.mul_smul_comm]
         simp only [List.nil_append]
         exact hψφ
@@ -277,30 +277,30 @@ lemma ι_timeOrder_superCommuteF_eq_time {φ ψ : 𝓕.CrAnStates}
   · intro x hx hpx
     simp_all [pb, hpx]
 
-lemma ι_timeOrder_superCommuteF_neq_time {φ ψ : 𝓕.CrAnStates}
+lemma ι_timeOrderF_superCommuteF_neq_time {φ ψ : 𝓕.CrAnStates}
     (hφψ : ¬ (crAnTimeOrderRel φ ψ ∧ crAnTimeOrderRel ψ φ)) (a b : 𝓕.CrAnAlgebra) :
     ι 𝓣ᶠ(a * [ofCrAnState φ, ofCrAnState ψ]ₛca * b) = 0 := by
-  rw [timeOrder_timeOrder_mid]
+  rw [timeOrderF_timeOrderF_mid]
   have hφψ : ¬ (crAnTimeOrderRel φ ψ) ∨ ¬ (crAnTimeOrderRel ψ φ) := by
     exact Decidable.not_and_iff_or_not.mp hφψ
   rcases hφψ with hφψ | hφψ
-  · rw [timeOrder_superCommuteF_ofCrAnState_ofCrAnState_not_crAnTimeOrderRel]
+  · rw [timeOrderF_superCommuteF_ofCrAnState_ofCrAnState_not_crAnTimeOrderRel]
     simp_all only [false_and, not_false_eq_true, false_or, mul_zero, zero_mul, map_zero]
     simp_all
   · rw [superCommuteF_ofCrAnState_ofCrAnState_symm]
     simp only [instCommGroup.eq_1, neg_smul, map_neg, map_smul, mul_neg, Algebra.mul_smul_comm,
       neg_mul, Algebra.smul_mul_assoc, neg_eq_zero, smul_eq_zero]
-    rw [timeOrder_superCommuteF_ofCrAnState_ofCrAnState_not_crAnTimeOrderRel]
+    rw [timeOrderF_superCommuteF_ofCrAnState_ofCrAnState_not_crAnTimeOrderRel]
     simp only [mul_zero, zero_mul, map_zero, or_true]
     simp_all
 
 /-!
 
-## Defining normal order for `FiedOpAlgebra`.
+## Defining time order for `FiedOpAlgebra`.
 
 -/
 
-lemma ι_timeOrder_zero_of_mem_ideal (a : 𝓕.CrAnAlgebra)
+lemma ι_timeOrderF_zero_of_mem_ideal (a : 𝓕.CrAnAlgebra)
     (h : a ∈ TwoSidedIdeal.span 𝓕.fieldOpIdealSet) : ι 𝓣ᶠ(a) = 0 := by
   rw [TwoSidedIdeal.mem_span_iff_mem_addSubgroup_closure] at h
   let p {k : Set 𝓕.CrAnAlgebra} (a : CrAnAlgebra 𝓕) (h : a ∈ AddSubgroup.closure k) := ι 𝓣ᶠ(a) = 0
@@ -314,11 +314,11 @@ lemma ι_timeOrder_zero_of_mem_ideal (a : 𝓕.CrAnAlgebra)
     match hc with
     | Or.inl hc =>
       obtain ⟨φa, φa', hφa, hφa', rfl⟩ := hc
-      simp only [ι_timeOrder_superCommuteF_superCommuteF]
+      simp only [ι_timeOrderF_superCommuteF_superCommuteF]
     | Or.inr (Or.inl hc) =>
       obtain ⟨φa, hφa, φb, hφb, rfl⟩ := hc
       by_cases heqt : (crAnTimeOrderRel φa φb ∧ crAnTimeOrderRel φb φa)
-      · rw [ι_timeOrder_superCommuteF_eq_time]
+      · rw [ι_timeOrderF_superCommuteF_eq_time]
         simp only [map_mul]
         rw [ι_superCommuteF_of_create_create]
         simp only [zero_mul]
@@ -326,11 +326,11 @@ lemma ι_timeOrder_zero_of_mem_ideal (a : 𝓕.CrAnAlgebra)
         · exact hφb
         · exact heqt.1
         · exact heqt.2
-      · rw [ι_timeOrder_superCommuteF_neq_time heqt]
+      · rw [ι_timeOrderF_superCommuteF_neq_time heqt]
     | Or.inr (Or.inr (Or.inl hc)) =>
       obtain ⟨φa, hφa, φb, hφb, rfl⟩ := hc
       by_cases heqt : (crAnTimeOrderRel φa φb ∧ crAnTimeOrderRel φb φa)
-      · rw [ι_timeOrder_superCommuteF_eq_time]
+      · rw [ι_timeOrderF_superCommuteF_eq_time]
         simp only [map_mul]
         rw [ι_superCommuteF_of_annihilate_annihilate]
         simp only [zero_mul]
@@ -338,18 +338,18 @@ lemma ι_timeOrder_zero_of_mem_ideal (a : 𝓕.CrAnAlgebra)
         · exact hφb
         · exact heqt.1
         · exact heqt.2
-      · rw [ι_timeOrder_superCommuteF_neq_time heqt]
+      · rw [ι_timeOrderF_superCommuteF_neq_time heqt]
     | Or.inr (Or.inr (Or.inr hc)) =>
       obtain ⟨φa, φb, hdiff, rfl⟩ := hc
       by_cases heqt : (crAnTimeOrderRel φa φb ∧ crAnTimeOrderRel φb φa)
-      · rw [ι_timeOrder_superCommuteF_eq_time]
+      · rw [ι_timeOrderF_superCommuteF_eq_time]
         simp only [map_mul]
         rw [ι_superCommuteF_of_diff_statistic]
         simp only [zero_mul]
         · exact hdiff
         · exact heqt.1
         · exact heqt.2
-      · rw [ι_timeOrder_superCommuteF_neq_time heqt]
+      · rw [ι_timeOrderF_superCommuteF_neq_time heqt]
   · simp [p]
   · intro x y hx hy
     simp only [map_add, p]
@@ -358,16 +358,16 @@ lemma ι_timeOrder_zero_of_mem_ideal (a : 𝓕.CrAnAlgebra)
   · intro x hx
     simp [p]
 
-lemma ι_timeOrder_eq_of_equiv (a b : 𝓕.CrAnAlgebra) (h : a ≈ b) :
+lemma ι_timeOrderF_eq_of_equiv (a b : 𝓕.CrAnAlgebra) (h : a ≈ b) :
     ι 𝓣ᶠ(a) = ι 𝓣ᶠ(b) := by
   rw [equiv_iff_sub_mem_ideal] at h
   rw [LinearMap.sub_mem_ker_iff.mp]
   simp only [LinearMap.mem_ker, ← map_sub]
-  exact ι_timeOrder_zero_of_mem_ideal (a - b) h
+  exact ι_timeOrderF_zero_of_mem_ideal (a - b) h
 
 /-- Time ordering on `FieldOpAlgebra`. -/
 noncomputable def timeOrder : FieldOpAlgebra 𝓕 →ₗ[ℂ] FieldOpAlgebra 𝓕 where
-  toFun := Quotient.lift (ι.toLinearMap ∘ₗ CrAnAlgebra.timeOrder) ι_timeOrder_eq_of_equiv
+  toFun := Quotient.lift (ι.toLinearMap ∘ₗ timeOrderF) ι_timeOrderF_eq_of_equiv
   map_add' x y := by
     obtain ⟨x, hx⟩ := ι_surjective x
     obtain ⟨y, hy⟩ := ι_surjective y
